Rec example done up to one coinduction issue

theories/ACCSExamples.v
@@ -1,24 +1,142 @@
-From Must Require Import ACCSInstance TransitionSystems Coin.
-From stdpp Require Import strings sets gmap base.
+From Must Require Import ACCSInstance TransitionSystems Coin Termination
+                         Must Completeness Soundness Equivalence.
+From stdpp Require Import strings sets gmap base gmultiset.
 From Coq Require Import Relations.
+From Coq Require Import Program.Equality.
+From Must Require Import Must.
 
-(* Tactic that looks for lts/lts_step assumptions and inverts them to
-  learn about the shape of the conclusion *)
-Ltac lts_inversion :=
-repeat match goal with
-| H : lts_step ?p ?a ?q |- _ => inversion H; subst; clear H
-| H : lts ?p ?a ?q |- _ => inversion H; subst; clear H
- end.
+
+Ltac lts_inversion := Termination.lts_inversion lts; try discriminate.
+Ltac step_tac := Termination.step_tac lts; simpl.
+Ltac term_tac := repeat step_tac.
+
+(*
+(* Parallel composition in ACCS is similar to the parallel composition of LTSs *)
+Lemma accs_parallel_sim (p q : proc) :
+  (p ∥ q) ≲ (p, q).
+Proof.
+revert p q. cofix hco. intros p q. constructor.
+intros α r Hstep. inversion Hstep; subst.
+- eexists (p2, q2); split.
+  + econstructor; simpl; eauto. now destruct μ.
+  + apply hco.
+- eexists; split.
+  + econstructor; simpl; eauto.
+  + apply hco.
+- eexists; split.
+  + econstructor; simpl; eassumption.
+  + apply hco.
+Qed.
+
+(* Parallel composition in ACCS with forwarders is similar to
+  the parallel composition of LTSs (with forwarder on one side) *)
+Lemma accs_fw_parallel_sim (p q : proc) (M : mb name):
+  ((p ∥ q) ▷ M) ≲ (p, (q ▷ M)).
+Proof.
+revert M p q. cofix hco. intros M p q. constructor.
+intros α r Hstep. inversion Hstep; subst.
+- inversion H3; subst.
+  + exists (p2, (q2, M)); split.
+    * eapply ParSync with (α1 := ActExt μ) (α2 := ActExt (co μ)); trivial.
+      -- destruct μ; simpl; trivial.
+      -- now constructor.
+    * apply hco.
+  + eexists; split.
+    * econstructor; simpl; eauto.
+    * apply hco.
+  + eexists; split.
+    * econstructor 2; simpl. constructor. eassumption.
+    * apply hco.
+- eexists; split.
+  + econstructor 2; simpl; constructor 2.
+  + apply hco.
+- eexists; split.
+  + econstructor 2; simpl; constructor 3.
+  + apply hco.
+- inversion H3; subst.
+  + exists (p2, (q, m)); split.
+    * apply ParSync with (α1 := ActExt (ActIn a))
+                          (α2 := ActExt (ActOut a)); simpl; eauto.
+      constructor.
+    * apply hco.
+  + exists (p, (q2, m)); split.
+    * econstructor 2; simpl. constructor. eassumption.
+    * apply hco.
+Qed.
+*)
+
+Derive Inversion_clear lts_inv with (forall p a q, lts p a q) Sort Prop.
+Derive Inversion_clear lts_step_inv with (forall p a q, lts_fw_step p a q)
+  Sort Prop.
+(*
+Lemma pr_nil_similar p : (pr_nil ∥ p) ≲ p.
+Proof.
+revert p. cofix hco. intro p.
+constructor. intros α q Hq. lts_inversion.
+- inversion H1.
+- inversion H3.
+- eexists; split; eauto.
+Qed.
+*)
+
+Hint Constructors lts_fw_step : lts.
+Hint Constructors lts : lts.
+Hint Unfold lts_step : lts.
+Hint Extern 0 => simpl : lts.
+
+(*
+Lemma pr_nil_fw_similar p M : (pr_nil ∥ p ▷ M) ≲ (p ▷ M).
+Proof.
+revert p M. cofix hco. intros p M.
+constructor. intros α q Hq. lts_inversion.
+- lts_inversion.
+  + inversion H1.
+  + inversion H4.
+  + eexists; split; eauto with lts.
+- eexists; split; eauto with lts.
+- eexists; split; eauto with lts.
+- lts_inversion.
+  + inversion H4.
+  + eexists; split; eauto with lts.
+Qed.
+
+Lemma parallel_output_mb_similar μ (q : proc) (M : mb name):
+  (!μ ∥ q  ▷ M) ≲ (q ▷ {[+ μ +]} ⊎ M).
+Proof.
+revert q M. cofix hco. intros q M.
+constructor. intros α r Hstep.
+inversion Hstep; subst; clear Hstep.
+- lts_inversion.
+  + inversion H1; subst. eexists; split; eauto.
+    * apply lts_fw_com. eauto.
+    * apply pr_nil_fw_similar.
+  + lts_inversion. eexists; split; eauto.
+    * apply lts_fw_out_mb.
+    * apply pr_nil_fw_similar.
+  + eexists; split; eauto.
+    now apply lts_fw_p.
+- eexists; split; eauto.
+  replace ({[+ μ +]} ⊎ ({[+ a +]} ⊎ m)) with ({[+ a +]} ⊎ ({[+ μ +]} ⊎ m));
+  [constructor| clear hco; multiset_solver].
+- eexists; split; eauto.
+  replace ({[+ μ +]} ⊎ ({[+ a +]} ⊎ M)) with ({[+ a +]} ⊎ ({[+ μ +]} ⊎ M));
+  [constructor| clear hco; multiset_solver].
+- lts_inversion.
+  + lts_inversion.
+  + exists (q2 ▷ {[+ μ +]} ⊎ m); split.
+    * replace ({[+ μ +]} ⊎ ({[+ a +]} ⊎ m)) with ({[+ a +]} ⊎ ({[+ μ +]} ⊎ m));
+      [now constructor| clear hco; multiset_solver].
+    * apply hco.
+Qed.
+
 
 Lemma parallel_output_terminate M a b : (!a ∥ !b ▷ M) ⤓.
 Proof.
 constructor. intros (p, M') Hl. inversion Hl; subst.
-- lts_inversion. discriminate.
-- decompose record Hl. lts_inversion.
+- repeat lts_inversion.
+- decompose record Hl. repeat lts_inversion.
 Qed.
-
-(* A tactic to try and prove termination *)
-Ltac term_tac := repeat(constructor; intros; lts_inversion).
+*)
 
 Example q_terminate : forall M, (!"a" ∥ (τ⋅ !"b" ⊕  τ⋅ !"c") ▷ M) ⤓.
 Proof. intro M. term_tac. Qed.
@@ -27,7 +145,7 @@ Lemma choice_copre_l p q: forall (M : mb name) X,
   {[τ⋅ p ⊕ τ⋅ q ▷ M]} ∪ X ⩽ p ▷ M.
 Proof.
 intros M X. eapply c_tau.
-- apply coin_union, coin_refl.
+- apply coin_union_l, coin_refl.
 - constructor. apply lts_choiceL. constructor.
 Qed.
 
@@ -35,40 +153,35 @@ Lemma choice_copre_r p q: forall (M : mb name) X,
   {[τ⋅ p ⊕ τ⋅ q ▷ M]} ∪ X ⩽ q ▷ M.
 Proof.
 intros M X. eapply c_tau.
-- apply coin_union, coin_refl.
+- apply coin_union_l, coin_refl.
 - constructor. apply lts_choiceR. constructor.
 Qed.
-
-(* faster than set set_solver *)
-Ltac set_tac :=
-(apply elem_of_union_r; set_tac) ||
-(apply elem_of_union_l; set_tac) ||
-now apply elem_of_singleton_2.
 
 Lemma choice_copre_rev p q: forall M X,
   {[ (p ▷ M); (q ▷ M) ]} ∪ X ⩽ τ⋅ p ⊕ τ⋅ q ▷ M.
 Proof.
 cofix hco.
 intros. split.
-- clear hco. intros (q', M') l. 
+- clear hco. intros (q', M') l.
   inversion_clear l.
-  + lts_inversion; apply coin_elem_of; set_tac.
-  + lts_inversion.
+  + repeat lts_inversion; apply coin_elem_of; set_tac.
+  + repeat lts_inversion.
 - intros Ht Hs.
   exfalso. eapply (lts_stable_spec2 (τ⋅ p ⊕ τ⋅ q ▷ M)).
   eexists. eapply lts_fw_p, lts_choiceL, lts_tau. assumption.
 - intros μ q' ps' H0 Hμ Hw. inversion Hμ; subst.
-  + lts_inversion.
-  + rewrite (union_difference_L {[p ▷ m; q ▷ m ]} ps'). apply hco.
-    clear hco.
-    intros p' mem%elem_of_union.
-    destruct mem as [hl%elem_of_singleton | hr%elem_of_singleton]; subst.
-    * apply Hw with (p ▷ {[+ a +]} ⊎ m). set_tac.
-      eapply wt_act. eapply (lts_fw_out_mb m). eapply wt_nil.
-    * apply Hw with (q ▷ {[+ a +]} ⊎ m). set_tac.
-      eapply wt_act. eapply (lts_fw_out_mb m). eapply wt_nil.
-  + rewrite (union_difference_L {[p ▷ {[+ a +]} ⊎ M; q ▷ {[+ a +]} ⊎ M]} ps'). apply hco.
-    clear hco.
+  + repeat lts_inversion.
+  + rewrite (union_difference_L {[p ▷ m; q ▷ m ]} ps').
+    * apply hco.
+    * clear hco.
+      intros p' mem%elem_of_union.
+      destruct mem as [hl%elem_of_singleton | hr%elem_of_singleton]; subst.
+      -- apply Hw with (p ▷ {[+ a +]} ⊎ m). set_tac.
+         eapply wt_act. eapply (lts_fw_out_mb m). eapply wt_nil.
+      -- apply Hw with (q ▷ {[+ a +]} ⊎ m). set_tac.
+         eapply wt_act. eapply (lts_fw_out_mb m). eapply wt_nil.
+  + rewrite (union_difference_L {[p ▷ {[+ a +]} ⊎ M; q ▷ {[+ a +]} ⊎ M]} ps').
+    apply hco. clear hco.
     intros p' mem%elem_of_union.
     destruct mem as [hl%elem_of_singleton | hr%elem_of_singleton]; subst.
     * apply Hw with (p ▷ M). set_tac.
@@ -76,45 +189,123 @@ intros. split.
     * eapply Hw with (q ▷ M). set_tac.
       eapply wt_act. eapply lts_fw_inp_mb. eapply wt_nil.
 - clear hco. intros Ht. constructor. intros (q', M') l.
-  inversion l; subst; lts_inversion; apply Ht; set_tac.
+  inversion l; subst; repeat lts_inversion; apply Ht; set_tac.
 Qed.
 
-(* TODO: avoid using h2 *)
+Hint Resolve coin_elem_of : coin.
+
+(* Recursively delete nil from term *)
+
+Fixpoint proc_absorb_nil (p : proc) := match p with
+| (p ∥ q) => let p' := proc_absorb_nil p in
+             let q' := proc_absorb_nil q in
+             if decide (p' = pr_nil) then q'
+             else if decide (q' = pr_nil) then p'
+             else p' ∥ q'
+| pr_rec n p => pr_rec n (proc_absorb_nil p)
+| g gp => g (gproc_absorb_nil gp)
+| p => p
+end
+with gproc_absorb_nil (gp : gproc) : gproc := match gp with
+| gpr_input a p => gpr_input a (proc_absorb_nil p)
+| gpr_tau p => gpr_tau (proc_absorb_nil p)
+| gpr_choice g1 g2 => let g1' := gproc_absorb_nil g1 in
+                      let g2' := gproc_absorb_nil g2 in
+                      if decide (g g1' = pr_nil) then g2'
+                      else if decide (g g2' = pr_nil) then g1'
+                      else gpr_choice g1' g2'
+| gp => gp
+end.
+
+(* Defining mutual induction principle for processes and guards *)
+Scheme proc_gproc_ind := Induction for proc Sort Prop
+  with gproc_proc_ind := Induction for gproc Sort Prop.
+
+(* TODO : also missing in VACCS *)
+Lemma cgr_choice_trans : forall p1 q1 p2 q2, g p1 ≡* g q1 -> g p2 ≡* g q2 -> 
+  pr_choice p1 p2 ≡* pr_choice q1 q2.
+Proof.
+intros. dependent induction H. 
+constructor.
+Admitted.
+
+
+
+Lemma proc_absorb_nil_cgr p : p ≡* proc_absorb_nil p.
+Proof.
+induction p using proc_gproc_ind with
+  (P0 := fun gp => g gp ≡* g (gproc_absorb_nil gp)); simpl; auto with *.
+- case decide; intro Heq; subst. {
+  transitivity (𝟘 ∥ p2).
+    + apply cgr_par_left. etrans; [eassumption|].
+      rewrite Heq. reflexivity.
+    + etrans; [|eassumption].
+      etrans; constructor.
+      * apply cgr_par_com.
+      * constructor.
+  }
+  case decide; intro Heq'. {
+  transitivity (p1 ∥ 𝟘).
+    + apply cgr_par_right. etrans; [eassumption|].
+      rewrite Heq'. reflexivity.
+    + etrans; [|eassumption]. constructor. constructor.
+  }
+  etrans; [apply cgr_par_left; eassumption|].
+  etrans; [apply cgr_par_right; eassumption|].
+  reflexivity.
+- induction IHp; [now repeat constructor| etrans; eassumption].
+- induction IHp; [now repeat constructor| etrans; eassumption].
+- induction IHp; [now repeat constructor| etrans; eassumption].
+- case decide; intro Heq; subst. {
+  transitivity (gpr_nil ⊕ g0).
+    + eapply cgr_choice_trans; [|reflexivity]. etrans; [eassumption|].
+      rewrite Heq. reflexivity.
+    + etrans; [constructor; apply cgr_choice_com|].
+      etrans; [constructor; apply cgr_choice_nil|]. assumption.
+  }
+  case decide; intro Heq'. {
+  transitivity (g ⊕ gpr_nil).
+    + apply cgr_choice_trans; [reflexivity|]. etrans; [eassumption|].
+      rewrite Heq'. reflexivity.
+    + etrans; [constructor; apply cgr_choice_nil|]. assumption.
+  }
+  apply cgr_choice_trans; assumption.
+Qed.
+
+
 Example code_hoisting_outputs : forall (M : mb name) X,
     {[ τ⋅ (!"a" ∥ !"b") ⊕ τ⋅ (!"a" ∥ !"c") ▷ M ]} ∪ X
       ⩽ !"a" ∥ (τ⋅ !"b" ⊕ τ⋅ !"c") ▷ M.
 Proof.
 cofix hco.
 intros M X. split.
-- intros q l. lts_inversion.
+- intros q l. repeat lts_inversion.
   + apply choice_copre_l.
   + apply choice_copre_r.
 - intros. exfalso.
   eapply (lts_stable_spec2 (!"a" ∥ (τ⋅ !"b" ⊕ τ⋅ !"c") ▷ M)); eauto.
   exists (!"a" ∥ !"b" ▷ M). eapply lts_fw_p, lts_parR, lts_choiceL, lts_tau.
 - intros μ q' ps' H0 Hμ Hw. inversion Hμ; subst.
-  + lts_inversion.
-  (* h2 : pas beau ! adhoc ; ACCS *)
+  + repeat lts_inversion.
     eapply h2.
     -- etrans. eapply t_step. eapply cgr_par_nil_rev.
        etrans. eapply t_step. eapply cgr_par_com. reflexivity.
     -- eapply (h2 (τ⋅ (pr_nil ∥ !"b") ⊕ τ⋅ (pr_nil ∥ !"c"))).
-      ++ symmetry.
-         etrans. eapply t_step. eapply cgr_choice.
-         eapply cgr_tau. eapply cgr_par_nil_rev.
-         eapply cgr_tau. eapply cgr_par_nil_rev.
-         etrans. eapply t_step. eapply cgr_choice.
-         eapply cgr_tau. eapply cgr_par_com.
-         eapply cgr_tau. eapply cgr_par_com. reflexivity.
+      ++ apply proc_absorb_nil_cgr.
       ++ assert (Hi : {[ (pr_nil ∥ !"b" ▷ M); (pr_nil ∥ !"c" ▷ M) ]} ⊆ ps'). {
           intros x mem%elem_of_union.
            destruct mem as [hl%elem_of_singleton | hr%elem_of_singleton]; subst.
-           eapply Hw. eapply elem_of_union. left. now eapply elem_of_singleton.
-           eapply wt_tau. eapply lts_fw_p. eapply lts_choiceL, lts_tau.
-           eapply wt_act. eapply lts_fw_p. eapply lts_parL, lts_output. eapply wt_nil.
-           eapply Hw. eapply elem_of_union. left. now eapply elem_of_singleton.
-           eapply wt_tau. eapply lts_fw_p. eapply lts_choiceR, lts_tau.
-           eapply wt_act. eapply lts_fw_p. eapply lts_parL, lts_output. eapply wt_nil.
+           - eapply Hw.
+            + eapply elem_of_union. left. now eapply elem_of_singleton.
+            + eapply wt_tau. apply lts_fw_p. apply lts_choiceL, lts_tau.
+              eapply wt_act. eapply lts_fw_p. eapply lts_parL, lts_output.
+              eapply wt_nil.
+           - eapply Hw.
+            + eapply elem_of_union. left. now eapply elem_of_singleton.
+            + eapply wt_tau. eapply lts_fw_p. eapply lts_choiceR, lts_tau.
+              eapply wt_act.
+              * eapply lts_fw_p. eapply lts_parL, lts_output. 
+              * eapply wt_nil.
          }
          eapply union_difference_L in Hi.
          rewrite Hi. eapply choice_copre_rev.
@@ -135,8 +326,663 @@ intros M X. split.
 - intros. eapply q_terminate.
 Qed.
 
-(* TODO: generalisation
-Example code_hoisting_gen a b c: forall (M : mb name) X,
-    {[ τ⋅ (a ∥ b) ⊕ τ⋅ (a ∥ c) ▷ M ]} ∪ X
-      ⩽ a ∥ (τ⋅ b ⊕ τ⋅ c) ▷ M.
+Section Omega.
+
+Definition omega := pr_rec 0 (pr_var 0). (* rec X. X *)
+
+Lemma omega_diverges : ¬ terminate omega.
+Proof.
+intro Ht. dependent induction Ht.
+apply (H0 omega).
+- term_tac.
+- trivial.
+Qed.
+
+Lemma omega_is_bottom p : {[omega]} ⩽ p.
+Proof.
+revert p.
+cofix hco. intros p.
+constructor.
+- intros q Hq. apply hco.
+- clear hco. intros Ht _. exfalso. apply omega_diverges, (Ht omega).
+  auto with *.
+- clear hco. intros a b c Ht _. exfalso.
+  eapply omega_diverges, cnv_terminate, (Ht omega).
+  auto with *.
+- clear hco. intros Ht. exfalso. apply omega_diverges, (Ht omega).
+  auto with *.
+Qed.
+
+End Omega.
+
+(*
+(* In ACCS, recursion unfolding steps are "invertible" τ steps *)
+Lemma rec_inv n p : forall μ p',
+  (pr_rec n p) ⟶{μ} p' <-> (p' = pr_subst n p (pr_rec n p) /\ μ = τ).
+Proof.
+intros μ p'. split; intro Hs.
+- now lts_inversion.
+- destruct Hs; subst. term_tac.
+Qed.
+
+
+(* Remark : proofs using the definition of must are not always difficult *)
+Lemma musts_choice (p q : gproc) (e : proc) : 
+  must (g p) e -> must (g q) e -> must (p ⊕ q) e.
+Proof.
+intros Hp Hq.
+dependent induction Hp; [now constructor|]. destruct Hq; [now constructor|].
+constructor 2.
+- trivial.
+- destruct ex as [[t1 t1'] H1']. dependent destruction H1'.
+  + exists (t1, t1'). apply ParLeft. constructor. assumption.
+  + exists (p ⊕ q ▷ t1'). apply ParRight. assumption.
+  + exists (t1, t1'). eapply ParSync; eauto.
+    constructor. assumption.
+- intros p' Hp'. inversion Hp'; subst.
+  + apply pt. assumption.
+  + apply pt0. assumption.
+- intros e' He'. eapply H0; trivial. now apply et0.
+- intros p' e' μ Hμ Hμ'. inversion Hμ'; subst.
+  + eapply com; eassumption.
+  + eapply com0; eassumption.
+Qed.
 *)
+
+
+Section Example_2_1.
+
+Definition unreliableW :=
+  pr_rec 0 ( τ⋅ ! "end" ⊕ ("data" ? (τ⋅ (! "work" ∥ pr_var 0) ⊕ τ⋅ ! "bye"))).
+
+Definition reliableW :=
+  pr_rec 0 (τ⋅ ! "end" ⊕ ("data" ? (! "work" ∥ pr_var 0))).
+
+
+Lemma reliableW_terminate M : (reliableW ▷ M) ⤓.
+Proof.
+(* By induction on the number of "data" in the mailbox. *)
+remember (multiplicity "data" M) as n. revert M Heqn.
+induction n; intros M Hs.
+- do 3 step_tac.
+  contradict Hs.
+  rewrite (multiplicity_disj_union {[+ "data" +]} m "data").
+  rewrite multiplicity_singleton. lia.
+- step_tac; step_tac; [step_tac|]. fold reliableW.
+  eapply terminate_preserved_by_eq.
+  + apply (IHn ( {[+"work" +]} ⊎ m)).
+    setoid_rewrite multiplicity_disj_union.
+    setoid_rewrite multiplicity_singleton_ne; [| by auto].
+    setoid_rewrite multiplicity_disj_union in Hs.
+    setoid_rewrite multiplicity_singleton in Hs. lia.
+  + (* This proof of equivalence can certainly be automated *)
+    eapply lts_oba_output_deter_inv.
+    * apply (lts_fw_out_mb m reliableW "work").
+    * term_tac.
+    * apply fw_eq_id_mb. etransitivity.
+      -- constructor. apply cgr_par_nil_rev.
+      -- constructor. apply cgr_par_com.
+Qed.
+
+Fixpoint add_work n p := match n with
+| O => p
+| S n => add_work n (!"work" ∥ p)
+end.
+
+Fixpoint add_data n m : mb name := 
+match n with
+| O => m
+| S n => add_data n ({[+ "data" +]} ⊎ m)
+end.
+
+Lemma add_work_comm n p :
+  add_work (S n) p = ! "work" ∥ (add_work n p).
+Proof.
+revert p; induction n; intro p; [trivial|].
+once unfold add_work at 2. fold add_work.
+rewrite <- IHn. trivial.
+Qed.
+
+
+Lemma add_work_inversion n :
+  (forall p q, p ↛[ActIn "work"] -> add_work n p ⟶ q ->
+    exists q', p ⟶ q' /\
+    q = add_work n q') /\
+  (forall p q μ, p ↛[ActIn "work"] -> lts (add_work n p) μ q ->
+    ((exists n1 n2, S (n1 + n2) = n /\ q = add_work n2 (𝟘 ∥ add_work n1 p) /\ μ = ActExt (ActOut "work")) \/
+    (exists q0, lts p μ q0 /\ q = add_work n q0 ))) /\
+  (forall p q μ, lts p μ q -> lts (add_work n p) μ (add_work n q)).
+Proof.
+induction n; (split; [|split]); intros p q.
+- intros Hs Hpq. eexists; split; eauto.
+- intros μ Hpq. right. eexists; split; eauto.
+- trivial.
+- intros Hs Hpq. rewrite add_work_comm in Hpq. lts_inversion.
+  + inversion H1. subst. clear H1. apply (proj1 (proj2 IHn)) in H2; trivial.
+    destruct H2 as [[n1 [n2 [Heq [Heq' HF]]]]|[q'[Hq' Heq]]];
+    subst; [discriminate|].
+    unfold lts_stable in Hs. simpl in Hs.
+    apply lts_set_spec1 in Hq'. multiset_solver.
+  + lts_inversion.
+  + apply (proj1 (proj2 IHn)) in H3; trivial.
+    destruct H3 as [[n1 [n2 [Heq [Heq' HF]]]]|[q'[Hq' Heq]]];
+    subst; [discriminate|].
+    exists q'; split; trivial. now rewrite add_work_comm.
+- simpl. intros μ Hs Hμ.
+  setoid_rewrite (add_work_comm n) in Hμ.
+  lts_inversion.
+  + inversion H1; subst. clear H1.
+    apply (proj1 (proj2 IHn)) in H4; trivial.
+    destruct H4 as [[n1 [n2 [Heq [Heq' HF]]]]|[q'[Hq' Heq]]]; subst;
+    [discriminate|].
+    apply lts_set_spec1 in Hq'. multiset_solver.
+  + lts_inversion. left. exists n; exists 0; repeat split; trivial. lia.
+  + apply (proj1 (proj2 IHn)) in H3; trivial. clear IHn.
+    destruct H3 as [[n1 [n2 [Heq [Heq' HF]]]]|[q'[Hq' Heq]]]; subst.
+    * left. exists n1; exists (S n2). repeat split; trivial; [lia|].
+      now rewrite add_work_comm.
+    * right; exists q'; split; trivial.
+      now setoid_rewrite (add_work_comm n).
+- intros μ Hμ. repeat rewrite (add_work_comm n).
+  apply lts_parR, IHn, Hμ.
+Qed.
+
+(* unused 
+Lemma parallel_output_preserve_termination a p M :
+ (forall q l, wt p l q -> ¬ In (ActIn a) l) -> (p  ▷ M) ⤓ -> (! a ∥ p ▷ M) ⤓.
+Proof.
+intros Hs Ht. dependent induction Ht generalizing M p Hs.
+constructor. intros q Hq.
+lts_inversion.
+- lts_inversion.
+  + inversion H3; subst. clear H3.
+    exfalso; apply (Hs q2 [ActIn a]); [|auto with *].
+    eapply wt_act; [|apply wt_nil]. assumption.
+  + lts_inversion.
+  + apply H0 with (q2 ▷ M).
+    * constructor; trivial.
+    * intros q l Hq. apply (Hs q l).
+      apply wt_tau with q2; assumption.
+    * trivial.
+- lts_inversion.
+  + lts_inversion.
+  + eapply H0 with (q2 ▷ m); trivial.
+    * now constructor.
+    * intros q l Hq Ha. apply (Hs q (ActIn a0 :: l)); [|auto with *].
+      eapply wt_act; eassumption.
+Qed.
+*)
+
+(* unused for now
+Lemma harmony_wt: ∀ (p q : proc) s,
+  (∃ r : proc, p ≡* r ∧ wt r s q) → ∃ r : proc, wt p s r ∧ r ≡* q.
+Proof.
+intros p q s [r [Heq Hr]]. dependent induction Hr generalizing p Heq.
+- eexists; split; eauto using wt_nil.
+- destruct (harmony_cgr p q τ) as [r [Hs Heqr]].
+  + exists p0. split; trivial.
+  + destruct (IHHr r Heqr) as [r' [Hr' Heqr']].
+    exists r'; split; trivial.
+    apply wt_tau with r; trivial.
+- destruct (harmony_cgr p q (ActExt μ)) as [r [Hs Heqr]].
+  + exists p0. split; trivial.
+  + destruct (IHHr r Heqr) as [r' [Hr' Heqr']].
+    exists r'; split; trivial.
+    apply wt_act with r; trivial.
+Qed.
+
+*)
+
+
+Lemma cgr_par_nil_l p : 𝟘 ∥ p ≡* p.
+Proof.
+eapply t_trans.
+- eapply t_step, cgr_par_com.
+- eapply t_step, cgr_par_nil.
+Qed.
+
+(* unused 
+
+Lemma output_no_ActIn p a:
+  (forall q l, wt p l q -> ¬ In (ActIn a) l) ->
+    (forall q l, wt (! a ∥ p) l q -> ¬ In (ActIn a) l).
+Proof.
+intros Hp q l Hwt.
+dependent induction Hwt; simpl.
+- tauto.
+- lts_inversion.
+  + inversion H1; subst. clear H1.
+    intro.
+    eapply (Hp q2 [ActIn a]); [|auto with *].
+    eapply wt_act; [|apply wt_nil]. eassumption.
+  + lts_inversion.
+  + eapply IHHwt; [|reflexivity].
+    intros q l Hl. eapply (Hp q l).
+    eapply wt_tau; [eassumption|]; assumption.
+- intros [Heq|HF].
+  + subst. lts_inversion; [lts_inversion|].
+    apply (Hp q2 [ActIn a]); [|auto with *].
+    eapply wt_act; [eassumption| apply wt_nil].
+  + lts_inversion.
+    * lts_inversion. destruct (harmony_wt p t s) as [r [Hr Heqr]].
+      -- exists (𝟘 ∥ p). split; trivial. symmetry; apply cgr_par_nil_l.
+      -- apply (Hp r s Hr HF).
+    * apply (IHHwt a q2); trivial.
+      intros q l Hl. intro Hal. apply (Hp q (μ :: l)); [|auto with *].
+      eapply wt_act; [eassumption|]; assumption.
+Qed.
+
+Lemma add_work_no_ActIn p n:
+  (forall q l, wt p l q -> ¬ In (ActIn "work") l) ->
+    (forall q l, wt (add_work n p) l q -> ¬ In (ActIn "work") l).
+Proof.
+intro Hp. induction n; trivial.
+rewrite add_work_comm.
+intros. eapply output_no_ActIn; eauto.
+Qed.
+
+Lemma add_work_terminate n : ∀ p M,
+ (forall q l, wt p l q -> ¬ In (ActIn "work") l) -> (p  ▷ M) ⤓ ->
+   (add_work n p ▷ M) ⤓.
+Proof.
+intros p M Hp Ht.
+induction n; trivial.
+rewrite add_work_comm.
+apply parallel_output_preserve_termination; [|apply IHn].
+apply add_work_no_ActIn, Hp.
+Qed.
+
+*)
+
+Ltac wt_inversion:=
+match goal with
+| H : wt ?p ?a ?q |- _ =>
+  inversion H; subst; clear H; repeat lts_inversion; simpl in *
+end;
+try match goal with
+| H : ?a ⊎ ?b = ∅ |- _ => contradict H; apply Lift.neq_multi_nil
+end;
+try discriminate; try tauto; auto with *.
+
+(* Tactic to handle assumptions about add_work *)
+Ltac add_tac := match goal with
+| H : (lts_step (add_work ?n _) ?μ ?q0) |- _ =>
+  apply add_work_inversion in H; try tauto;
+  decompose [and or ex] H; subst; clear H; try discriminate
+| H : (lts (add_work ?n _) ?μ ?q0) |- _ => 
+  apply add_work_inversion in H; try tauto;
+  decompose [and or ex] H; subst; clear H; try discriminate
+end;
+repeat match goal with
+| H : ActExt ?A = ActExt ?B |- _ => inversion H; subst end.
+
+Lemma add_work_end_terminate M w : (add_work w (!"end") ▷ M) ⤓.
+Proof.
+constructor. intros q Hq. inversion Hq; subst;
+(add_tac; [lts_inversion|term_tac]).
+Qed.
+
+(* Strengthening *)
+Lemma add_work_reliableW_terminate M w : (add_work w reliableW ▷ M) ⤓.
+Proof.
+(* By induction on the number of "data" in the mailbox. *)
+remember (multiplicity "data" M) as n. revert M w Heqn.
+induction n; intros M w Hs.
+- constructor. intros q Hq; lts_inversion;
+  (add_tac; [lts_inversion |term_tac]).
+  constructor. intros q Hq. lts_inversion;
+  (add_tac; [repeat lts_inversion |term_tac]).
+  + apply add_work_end_terminate. (* end *)
+  + contradict Hs.
+    rewrite (multiplicity_disj_union {[+ "data" +]} m "data").
+    rewrite multiplicity_singleton. lia.
+- constructor. intros q Hq; lts_inversion; (add_tac; [lts_inversion |term_tac]).
+  constructor. intros q Hq; lts_inversion;
+    (add_tac; [repeat lts_inversion |term_tac]).
+  + apply add_work_end_terminate. (* end *)
+  + fold reliableW. apply (IHn m (S w)).
+    rewrite (multiplicity_disj_union {["data"]} m), multiplicity_singleton in Hs.
+    now inversion Hs.
+Qed.
+
+(* can be deduced from add_work_reliableW_terminate? *)
+
+Lemma add_data_comm a n m :
+ {[+ a +]} ⊎ add_data n m = add_data n ({[+ a +]} ⊎ m).
+Proof.
+revert m. induction n; intros m; simpl; [|rewrite IHn; f_equal]; multiset_solver.
+Qed.
+
+
+(* TODO: ⟹ should have lower priority than ∥ *)
+Lemma wt_par_l p q r s : p ⟹[s] q -> (r ∥ p) ⟹[s] (r ∥ q).
+Proof.
+intro Ht. induction Ht.
+- apply wt_nil.
+- apply wt_tau with (r ∥ q); trivial.
+  apply lts_parR; trivial.
+- apply wt_act with (r ∥ q); trivial.
+  apply lts_parR; trivial.
+Qed.
+
+
+Lemma lts_fw_par_l p q α M M' r:
+  lts_step (p ▷ M) α (q ▷ M')->
+    lts_step (r ∥ p ▷ M) α (r ∥ q ▷ M').
+Proof.
+intro Hs. inversion Hs; subst.
+- now apply lts_fw_p, lts_parR.
+- apply (lts_fw_out_mb M' (r ∥ q) a).
+- apply (lts_fw_inp_mb M (r ∥ q) a).
+- apply (lts_fw_com M' (r ∥ p) a (r ∥ q)), lts_parR. trivial.
+Qed.
+
+Lemma wt_par_fw_l p q M M' r s:
+  (p ▷ M) ⟹[s] (q ▷ M')->
+    (r ∥ p ▷ M) ⟹[s] (r ∥ q ▷ M').
+Proof.
+intro Ht. dependent induction Ht.
+- apply wt_nil.
+- destruct q0 as [q0 M0].
+  apply wt_tau with (r ∥ q0 ▷ M0).
+  + now apply lts_fw_par_l.
+  + now apply IHHt.
+- destruct q0 as [q0 M0].
+  apply wt_act with (r ∥ q0 ▷ M0).
+  + now apply lts_fw_par_l.
+  + now apply IHHt.
+Qed.
+
+Fixpoint add_zeros n p := match n with
+| O => p
+| S n => add_zeros n (𝟘 ∥ p)
+end.
+
+Lemma add_zeroes_comm n p :
+  add_zeros (S n) p = 𝟘 ∥ (add_zeros n p).
+Proof.
+revert p; induction n; intro p; [trivial|].
+once unfold add_zeros at 2. fold add_zeros.
+rewrite <- IHn. trivial.
+Qed.
+
+Lemma add_zeros_lts : forall n p q α,
+  lts p α q <-> lts (add_zeros n p) α (add_zeros n q).
+Proof.
+induction n; intros p q α; trivial.
+do 2 rewrite add_zeroes_comm. rewrite IHn. split; intro Hpq.
+- apply lts_parR, Hpq.
+- lts_inversion.
+  + inversion H3.
+  + inversion H2.
+  + trivial.
+Qed.
+
+Lemma add_work_plus x x0 p :
+  add_work (x + x0) p = add_work x (add_work x0 p).
+Proof.
+revert x0 p. induction x as [|x]; intros x0 p; trivial.
+simpl. now rewrite IHx, <- add_work_comm.
+Qed.
+
+Local Instance Proper_par : Proper (cgr ==> cgr ==> cgr) (fun x y => x ∥ y).
+Proof.
+intros p p' Hp q q' Hq. 
+eapply t_trans.
+- apply cgr_par_right, Hq.
+- apply cgr_par_left, Hp.
+Defined.
+
+
+Lemma add_zeros_cgr p z : add_zeros z p ≡* p.
+Proof.
+revert p; induction z; intro p; simpl.
+- reflexivity.
+- rewrite IHz. apply cgr_par_nil_l.
+Qed.
+
+
+Global Instance Reflexive_cgr : Reflexive cgr.
+Proof. intro x. apply t_step, cgr_refl. Defined.
+
+Local Instance Proper_add_work : Proper (eq ==> cgr ==> cgr) add_work.
+Proof.
+intros n n' Hn. subst n'. induction n; intros p p' Hp; trivial.
+do 2 rewrite add_work_comm. apply Proper_par; auto with *.
+Defined.
+
+Lemma add_work_par_comm x p1 p2 :
+  add_work x (p1 ∥ p2) ≡* p1 ∥ add_work x p2.
+Proof.
+revert p1 p2. induction x as [|x]; intros p1 p2; simpl; trivial.
+- reflexivity.
+- repeat rewrite IHx.
+  eapply t_trans; [ apply t_step; symmetry; apply cgr_par_ass|].
+  eapply t_trans; [|apply t_step, cgr_par_ass].
+  apply t_step. apply cgr_par.
+  + apply cgr_par_com.
+  + reflexivity.
+Qed.
+
+Lemma add_zeros_par_comm z p1 p2 :
+  add_zeros z (p1 ∥ p2) ≡* p1 ∥ add_zeros z p2.
+Proof.
+revert p1 p2. induction z as [|x]; intros p1 p2; simpl; trivial.
+- reflexivity.
+- repeat rewrite IHx.
+  eapply t_trans; [ apply t_step; symmetry; apply cgr_par_ass|].
+  eapply t_trans; [|apply t_step, cgr_par_ass].
+  apply t_step. apply cgr_par.
+  + apply cgr_par_com.
+  + reflexivity.
+Qed.
+
+(* After n unfolding and n "data" received, n "work" have been produced *)
+Lemma unreliable_add_work_add_data_terminate z n M :
+  (add_zeros z unreliableW ▷ add_data n M) ⟹ (add_zeros z (add_work n (! "end")) ▷ M).
+Proof.
+revert z M. induction n as [|n]; intros z M; simpl.
+- eapply wt_tau; [constructor; apply add_zeros_lts; term_tac|].
+  eapply wt_tau; [constructor; apply add_zeros_lts; term_tac|]. apply wt_nil.
+- eapply wt_tau; [constructor; apply add_zeros_lts; term_tac|]. simpl.
+  fold unreliableW. eapply wt_tau.
+  + setoid_rewrite <- (add_data_comm "data" n M).
+    apply lts_fw_com, add_zeros_lts, lts_choiceR. constructor.
+  + apply wt_tau with (add_zeros z (! "work" ∥ unreliableW) ▷ add_data n M).
+    * apply lts_fw_p, add_zeros_lts, lts_choiceL. constructor.
+    * setoid_rewrite add_work_comm.
+      induction z.
+      -- apply wt_par_fw_l. apply (IHn 0).
+      -- do 2 rewrite add_zeroes_comm. apply wt_par_fw_l, IHz.
+Qed.
+
+Lemma reliableW_consume_data n M :
+  (add_work n reliableW ▷ ({[+ "data"+]} ⊎ M))
+    ⟹ (add_work n (! "work" ∥ reliableW) ▷ M).
+Proof.
+  eapply wt_tau.
+  - constructor. apply add_work_inversion. constructor.
+  - simpl. fold reliableW. eapply wt_tau; [|apply wt_nil].
+    simpl. apply (lts_fw_com M).
+    apply add_work_inversion. apply lts_choiceR. constructor.
+Qed.
+
+Lemma reliableW_stable_work : reliableW ↛[ActIn "work"].
+Proof. now vm_compute. Qed.
+
+
+Lemma add_work_zero x x0 p :
+  add_work (x + x0) p ≡* add_work x0 (𝟘 ∥ add_work x p).
+Proof.
+replace (x + x0) with (x0 + x) by lia.
+rewrite add_work_plus. apply Proper_add_work. trivial.
+symmetry. eapply t_trans.
+- eapply t_step, cgr_par_com.
+- eapply t_step, cgr_par_nil.
+Qed.
+
+Require Import Must.
+
+Axiom FF : False.
+Ltac cheat := exfalso; apply FF.
+
+Example unreliable_reliable :
+ unreliableW ⊑ reliableW.
+Proof. 
+apply soundness, alt_set_singleton_iff, eqx.
+(* generalisation *)
+enough (Ht : forall n z (M :  mb name) X,
+  {[add_zeros z unreliableW ▷ add_data n M]} ∪ X ⩽ add_work n reliableW ▷ M). {
+  replace ({[unreliableW ▷ (∅ : mb name)]}) with
+          ({[unreliableW ▷ add_data 0 ∅ ]} ∪ ∅ : gset (proc * mb name))
+          by (simpl; set_solver).
+  apply (Ht 0 0 ∅ ∅).
+  }
+cofix hco. intros n z M X.
+assert(Hrs := reliableW_stable_work).
+constructor.
+(* A. stable by τ *)
+- intros q Hq. lts_inversion; add_tac; lts_inversion.
+  simpl. fold reliableW. constructor.
+  (* A' : stable by τ *)
+  + intros q Hq. lts_inversion; add_tac; repeat lts_inversion.
+    * (* → add_work n (! "end") ▷ M *)
+      apply h2 with (add_zeros z (add_work n (! "end")));
+      [by apply add_zeros_cgr|].
+      apply co_preserved_by_wt_nil with (add_zeros z unreliableW ▷ add_data n M);
+      [|refine (coin_union_l _ _ _ (coin_refl))].
+      apply unreliable_add_work_add_data_terminate.
+    * (* Loop back on coinduction hypothesis, with one more !"work" *)
+      apply (hco (S n)).
+  + (* B' : weak transitions outputs *)
+    clear hco. intros Ht Hs.
+    contradict Hs. apply lts_stable_spec2.
+    exists (add_work n (!"end") ▷ M). constructor. apply add_work_inversion.
+    term_tac.
+  + (* C' : Weak termination sets *)
+    intros μ q' ps' Hμ1 Hμ2 Hwt. lts_inversion.
+    * add_tac.
+      -- (* output "work" *)
+        eapply h2 with
+          (𝟘 ∥ add_work (x + x0)
+                        (τ⋅ ! "end" ⊕ ("data" ? (! "work" ∥ reliableW)))).
+       { replace (x + x0) with (x0 + x) by lia. 
+         rewrite add_work_par_comm, add_work_plus. reflexivity. }
+        apply co_preserved_by_wt_nil with (𝟘 ∥ add_work (x + x0) reliableW ▷ M).
+        ++ eapply wt_tau; [|apply wt_nil].
+           constructor. constructor. apply add_work_inversion; term_tac.
+        ++ assert(Hin : (add_zeros (S z) unreliableW ▷ add_data (x + x0) M) ∈ ps').
+          {
+            clear hco. (* needed to avoid set_tac to use hco *)
+            eapply Hwt with (p := add_zeros z unreliableW ▷ add_data (S (x + x0)) M)
+            ; [ set_tac|].
+            simpl. rewrite <- add_data_comm.
+            eapply wt_tau with
+              (add_zeros z (τ⋅ ! "end" ⊕
+                           ("data" ? (τ⋅ (! "work" ∥ unreliableW) ⊕
+                                      τ⋅ ! "bye")))
+               ▷ {[+ "data" +]} ⊎ add_data (x + x0) M);
+              [apply lts_fw_p; apply add_zeros_lts; constructor|].
+            eapply wt_tau with (add_zeros z (τ⋅ (! "work" ∥ unreliableW) ⊕ τ⋅ ! "bye")
+                                ▷ add_data (x + x0) M);
+            [apply lts_fw_com, add_zeros_lts, lts_choiceR, lts_input|].
+            eapply wt_tau with (add_zeros z (! "work" ∥ unreliableW), add_data (x + x0) M);
+            [eapply lts_fw_p; apply add_zeros_lts; do 2 constructor|].
+            eapply wt_act; [|apply wt_nil].
+            apply lts_fw_p, add_zeros_lts. do 2 constructor.
+          }
+          apply union_difference_singleton_L in Hin. rewrite Hin.
+          apply h2 with (add_work (x + x0) reliableW); [|apply hco].
+          symmetry. apply cgr_par_nil_l.
+      -- lts_inversion; lts_inversion.
+         (* input "data" *)
+         eapply co_preserved_by_wt_nil with (add_work n reliableW ▷ ({["data"]} ⊎ M)).
+         2 : { eapply hco; eauto. constructor. }
+         apply reliableW_consume_data.
+    * apply co_preserved_by_wt_nil with (add_work n reliableW ▷ m).
+     -- eapply wt_tau; [|apply wt_nil].
+        constructor. eapply add_work_inversion. constructor.
+     -- assert(Hin : (add_zeros z  unreliableW ▷ add_data n m) ∈ ps'). {
+        clear hco. (* needed to avoid set_tac to use hco *)
+        eapply Hwt with (p := add_zeros z unreliableW
+                         ▷ add_data n ({[+ a +]} ⊎ m)); [ set_tac|].
+        rewrite <- add_data_comm. eapply wt_act;
+        [apply lts_fw_out_mb| apply wt_nil].
+        }
+        apply union_difference_singleton_L in Hin. rewrite Hin.
+        apply hco.
+    * apply co_preserved_by_wt_nil with (add_work n reliableW ▷ {[+ a +]} ⊎ M).
+     -- eapply wt_tau; [|apply wt_nil].
+        constructor. eapply add_work_inversion. constructor.
+     -- assert(Hin : (add_zeros z unreliableW ▷ add_data n ({[+ a +]} ⊎ M)) ∈ ps'). {
+        clear hco. (* needed to avoid set_tac to use hco *)
+        eapply Hwt with (p := add_zeros z unreliableW ▷ add_data n M); [ set_tac|].
+        rewrite <- add_data_comm. eapply wt_act;
+        [apply lts_fw_inp_mb|apply wt_nil].
+        }
+        apply union_difference_singleton_L in Hin. rewrite Hin.
+        apply hco.
+  + clear hco. intros _. clear X.
+    apply terminate_preserved_by_lts_tau with (add_work n reliableW ▷ M).
+    * apply add_work_reliableW_terminate.
+    * constructor. apply add_work_inversion. term_tac.
+(* B. Weak transitions to stable states preserve output inclusion *)
+- clear hco. intros Ht Hs.
+  destruct Hs as [Hs _]. simpl in Hs.
+  (* Easy, the right-hand side is stable. *)
+  assert (Htau : (add_work n reliableW) ⟶
+          (add_work n (τ⋅ ! "end" ⊕ ("data" ? (! "work" ∥ reliableW))))).
+  { apply add_work_inversion. constructor. }
+  contradict Hs. unfold proc_stable. apply lts_set_spec1 in Htau.
+  intro Heq; rewrite Heq in Htau. now apply elem_of_empty in Htau.
+(* C. Weak termination sets *)
+- intros μ q' ps' Hμ1 Hμ2 Hwt. inversion Hμ2; subst.
+  + destruct n as [|n]; [clear hco; lts_inversion|].
+    add_tac; [| clear hco; lts_inversion]. clear Hμ2.
+    assert(Hin : (add_zeros (S z) unreliableW ▷ add_data (x0 + x) M) ∈ ps'). {
+      clear hco. (* needed to avoid set_tac to use hco *)
+      apply Hwt with (p := add_zeros z unreliableW ▷ add_data (S (x + x0)) M);
+      [ simpl; set_solver|].
+      apply wt_tau with
+        (add_zeros z (τ⋅ ! "end" ⊕
+        ("data" ? (τ⋅ (! "work" ∥ unreliableW) ⊕ τ⋅ ! "bye")))
+         ▷ add_data (S (x + x0)) M); [apply lts_fw_p, add_zeros_lts; term_tac|].
+      setoid_rewrite <- add_data_comm.
+      apply wt_tau with (add_zeros z (τ⋅(! "work" ∥ unreliableW) ⊕ τ⋅! "bye")
+                         ▷ add_data (x + x0) M);
+      [apply lts_fw_com, add_zeros_lts, lts_choiceR; constructor|].
+      eapply wt_tau with (add_zeros z (! "work" ∥ unreliableW) ▷ add_data (x + x0) M);
+      [apply lts_fw_p, add_zeros_lts, lts_choiceL; constructor
+      |eapply wt_act; [|apply wt_nil]].
+      simpl. rewrite Nat.add_comm. apply lts_fw_p, add_zeros_lts. term_tac.
+    }
+    apply union_difference_singleton_L in Hin. rewrite Hin.
+    apply h2 with (add_work (x0 + x) reliableW); [|apply (hco (x0 + x) (S z))].
+    clear hco. (* ici? *)
+    rewrite add_work_par_comm, add_work_plus.
+    symmetry. apply cgr_par_nil_l.
+  + assert(Hin : (add_zeros z unreliableW ▷ add_data n m) ∈ ps'). {
+      clear hco. (* needed to avoid set_tac to use hco *)
+      eapply Hwt with (p := add_zeros z unreliableW ▷ add_data n ({[+ a +]} ⊎ m))
+      ; [ set_tac|].
+      eapply wt_act; [| apply wt_nil].
+      replace (add_data n ({[+ a +]} ⊎ m)) with ({[+ a +]} ⊎ (add_data n m));
+      [term_tac|]. apply add_data_comm.
+    }
+    apply union_difference_singleton_L in Hin. rewrite Hin.
+    apply hco.
+  + assert(Hin : (add_zeros z unreliableW ▷ add_data n ({[+a+]} ⊎ M)) ∈ ps'). {
+      clear hco.
+      eapply Hwt with (p := add_zeros z unreliableW ▷ add_data n M); [ set_tac|].
+      eapply wt_act.
+      apply lts_fw_inp_mb.
+      replace  ({[+ a +]} ⊎ (add_data n M)) with (add_data n ({[+ a +]} ⊎ M));
+      [term_tac|]. now rewrite add_data_comm.
+    }
+    apply union_difference_singleton_L in Hin. rewrite Hin.
+    apply hco.
+(* D. Termination on the left implies termination on the right *)
+- intros. apply add_work_reliableW_terminate.
+Qed.
+
+End Example_2_1.
